Work on proofs

type_safety.v
@@ -18,37 +18,122 @@ Proof.
     + apply IHtd; assumption.
 Qed.
 
-(* all free and bound variables *)
-Fixpoint vars_in_exp (e_5:exp) : list var :=
-  match e_5 with
-  | (exp_var var5) => (cons var5 nil)
-  | (exp_int word5) => nil
-  | (exp_load e1 e2 endian5 nat5) => (app (vars_in_exp e1) (vars_in_exp e2))
-  | (exp_store e1 e2 endian5 nat5 e3) => (app (vars_in_exp e1)
-                                              (app (vars_in_exp e2) (vars_in_exp e3)))
-  | (exp_binop e1 bop5 e2) => (app (vars_in_exp e1) (vars_in_exp e2))
-  | (exp_unop uop5 e1) => ((vars_in_exp e1))
-  | (exp_cast cast5 nat5 e) => ((vars_in_exp e))
-  | (exp_let var5 e1 e2) => (app (vars_in_exp e1) (cons var5 (vars_in_exp e2)))
-  | (exp_unk string5 type5) => nil
-  | (exp_ite e1 e2 e3) => (app (vars_in_exp e1) (app (vars_in_exp e2) (vars_in_exp e3)))
-  | (exp_ext nat1 nat2 e) => (vars_in_exp e)
-  | (exp_concat e1 e2) => (app (vars_in_exp e1) (vars_in_exp e2))
-end.
-
 Lemma in_list_minus : forall {A} (l l' : list A) (e : A) {dec},
-    In e (list_minus dec l l') -> In e l.
-  intros A l l' e dec e_in.
+    In e (list_minus dec l l') <-> In e l /\ ~In e l'.
+  intros A l l' e dec.
+  split.
+  intro e_in.
   induction l.
   - simpl in e_in; contradiction.
   - simpl in e_in.
     simpl.
+    constructor.
     destruct (list_mem dec a l').
-    + apply IHl in e_in; right; assumption.
+    + apply IHl in e_in; destruct e_in.
+      constructor; try right; assumption.
     + destruct e_in.
-      * left; assumption.
+      * constructor. try left; assumption.
       * right; apply IHl; assumption.
+    + unfold list_mem in e_in.
+      destruct (in_dec dec a l').
+      tauto.
+      destruct e_in.
+      * rewrite <- H.
+        assumption.
+      * tauto.
+  - intro conj; destruct conj as [in_l nin_l'].
+    induction l.
+    * tauto.
+    * simpl.
+      unfold list_mem.
+      destruct (in_dec dec a l'); destruct (dec e a).
+      -- rewrite e0 in nin_l'.
+         tauto.
+      -- destruct in_l.
+         ++ symmetry in H; contradiction.
+         ++ apply IHl in H; assumption.
+      -- rewrite e0; simpl; auto.
+      -- right; apply IHl.
+         destruct in_l.
+         ++ symmetry in H; contradiction.
+         ++ assumption.
+(* TODO: clean up proof *)
 Qed.
+
+Definition var_id : var -> id :=
+(fun v : var => match v with
+                | var_var id0 _ => id0
+                end).
+
+Lemma typ_gamma_remove_var : forall g x g', typ_gamma (g ++ x :: g') -> typ_gamma (g ++ g').
+Proof.
+  intros g x g'; revert g g' x.
+  induction g as [| x g].
+  - simpl.
+    intros g' x txg'.
+    inversion txg'; assumption.
+  -  simpl.
+     intros g' x0 txgxn.
+     inversion txgxn as [G | G id t nin tgxn x_eq_x].
+     apply IHg in tgxn.
+     fold var_id in nin.
+     apply tg_cons.
+     fold var_id.
+     rewrite map_app.
+     rewrite map_app in nin.
+     simpl in nin.
+     intro nin'.
+     apply in_app_or in nin'.
+     apply nin.
+     apply in_or_app.
+     destruct nin'.
+     left; assumption.
+     right; right; assumption.
+     assumption.
+Qed.
+
+(*
+Ltac unique_suffices_type_exp_base :=
+match goal with
+    | [ H_tG : typ_gamma ?G, H_G_eq : ?G = ?x :: ?g |- _ ] =>
+      destruct H_tG; inversion H_G_eq;
+        match goal with
+        | [ H_g_eq : ?G = g |- _ ] =>
+          rewrite H_g_eq in H_tG;
+            apply t_int;
+            assumption
+        end
+    end.
+
+Lemma unique_suffices_type_exp : forall (g g' : gamma) x e t,
+    In x (g ++ g')->
+    type_exp (g ++ x::g') e t ->
+    type_exp (g ++ g') e t.
+Proof.
+  intros g g' x e t x_in_g xg_te.
+  remember (g ++ x :: g') as gxg'.
+  induction xg_te.
+  - destruct H0; inversion Heqgxg'.
+    elim (app_cons_not_nil g g' x); assumption.
+    destruct (eq_var (var_var id5 t) x).
+    + rewrite <- e in x_in_g.
+      apply t_var.
+      * apply x_in_g.
+      * apply H0.
+    + rewrite Heqxg in H.
+      destruct H.
+      * elim n; symmetry; apply H.
+      * apply t_var; assumption.
+  - unique_suffices_type_exp_base.
+  - apply (t_load _ e1 e2 ed sz nat5); auto.
+  - apply (t_store _ e1 e2 ed sz e3); auto.
+  - apply t_aop; auto.
+  - apply (t_lop _ e1 lop5 e2 sz); auto.
+  - apply t_uop; auto.
+  - apply (t_cast _ _ _ _ nat5); auto.
+  - apply t_let; auto.
+    
+
 
 Lemma fv_impl_exp_v : forall x e, In x (fv_exp e) -> In x (vars_in_exp e).
   intros x e.
@@ -65,8 +150,7 @@ Lemma fv_impl_exp_v : forall x e, In x (fv_exp e) -> In x (vars_in_exp e).
   - apply in_app_or in H.
     firstorder.
 Qed.
-
-Definition var_id := (fun v => match v with var_var id _ => id end).
+*)
 
 Lemma type_exp_typ_gamma : forall g e t, type_exp g e t -> typ_gamma g.
 Proof.
@@ -105,16 +189,317 @@ Proof.
   - intros g HeqG tGw.
     apply (t_cast _ _ _ _ nat5); auto.
   - intros g HeqG tGw.
-    apply t_let.
-    + apply IHet1; assumption.
-    + rewrite app_comm_cons.
-      apply (IHet2 (var_var id5 t :: g)).
-      * rewrite <- app_comm_cons.
-        rewrite HeqG.
-        reflexivity.
-      * rewrite <- app_comm_cons.
-        apply tg_cons.
-        -- 
+    apply t_let; auto.
+  - intros g HeqG tGw.
+    apply t_unknown; auto.
+  - intros g HeqG tGw.
+    apply t_ite; auto.
+  - intros g HeqG tGw.
+    apply (t_extract _ _ _ _ sz); auto.
+  - intros g HeqG tGw.
+    apply t_concat; auto.
+Qed.
+
+Ltac subst_lfv_rec_case in_y_subst :=
+  simpl;
+  simpl in in_y_subst;
+  solve [firstorder
+        | try apply in_or_app;
+          apply in_app_or in in_y_subst;
+          destruct in_y_subst as [in_subst_es_1 | in_y_subst];
+          firstorder;
+          subst_lfv_rec_case in_y_subst
+        | right; subst_lfv_rec_case in_y_subst].
+
+Lemma subst_lfv_notin_e1 : forall x y e1 e2,
+    ~ In y (lfv_exp e1) ->
+    In y (lfv_exp (letsubst_exp e1 x e2)) ->   In y (lfv_exp e2).
+Proof.
+  intros x y e1 e2 lfv_e1_nin in_y_subst_e1.
+  induction e2.
+  all: try contradiction.
+  all: auto.
+  all: try subst_lfv_rec_case in_y_subst_e1.
+  - simpl in in_y_subst_e1.
+    destruct (eq_letvar letvar5 x).
+    +  contradiction.
+    + assumption.
+  - simpl.
+    simpl in in_y_subst_e1.
+    apply in_or_app.
+    apply in_app_or in in_y_subst_e1.
+    destruct in_y_subst_e1 as [in_subst_es_1 | in_y_subst].
+    firstorder.
+    right.
+    destruct (eq_letvar letvar5 x).
+    assumption.
+    apply in_list_minus in in_y_subst; destruct in_y_subst.
+    apply (in_list_minus (lfv_exp e2_2) (letvar5 :: nil) y).
+    constructor.
+    + auto.
+    + assumption.
+Qed.
+
+Lemma subst_lfv : forall x y e1 e2,
+    In y (lfv_exp (letsubst_exp e1 x e2)) -> In y (lfv_exp e1) \/  In y (lfv_exp e2).
+Proof.
+  intros x y e1 e2 in_y_subst_e1.
+  destruct (in_dec eq_letvar y (lfv_exp e1)).
+  - left; assumption.
+  - right; apply (subst_lfv_notin_e1 x y e1 e2); assumption.
+Qed.
+
+Ltac apply_all e t:=
+  repeat match goal with
+         | [ H : forall _ : t, _ |- _ ] =>
+           specialize (H e)
+         end.
+
+Ltac subst_lfv_neq_rec_case :=
+  intros e1 x_nin_lfv_e1 in_y_subst_e1;
+  simpl in in_y_subst_e1;
+  apply_all e1 exp;
+  repeat (apply in_app_or in in_y_subst_e1;
+          destruct in_y_subst_e1 as [in_subst_es_1 | in_y_subst_e1];
+          try tauto).
+
+Lemma subst_lfv_neq : forall x y e1 e2,
+    ~ In x (lfv_exp e1) ->
+    In y (lfv_exp (letsubst_exp e1 x e2)) -> ~ y = x.
+Proof.
+  intros x y e1 e2 x_nin_lfv_e1 in_y_subst_e1 x_eq_y.
+  rewrite x_eq_y in in_y_subst_e1.
+  generalize dependent e1.
+  induction e2.
+  all: try contradiction.
+  all: auto.
+  all: try solve [subst_lfv_neq_rec_case].
+  - intros e1 x_nin_lfv_e1 in_y_subst_e1.
+    simpl in in_y_subst_e1.
+    destruct (eq_letvar letvar5 x).
+    + contradiction.
+    + destruct in_y_subst_e1.
+      * contradiction.
+      * tauto.
+  - intros e1 x_nin_lfv_e1 in_y_subst_e1.
+    simpl in in_y_subst_e1.
+    apply in_app_or in in_y_subst_e1.
+    destruct in_y_subst_e1 as [in_subst_es_1 | in_y_subst].
+    + firstorder.
+    + apply (IHe2_2 e1).
+      * assumption.
+      * 
+   - subst_lfv_neq_rec_case.
+
+intros e1 x_nin_lfv_e1 in_y_subst_e1.
+      simpl in in_y_subst_e1.
+      apply_all e1 exp.
+      apply in_app_or in in_y_subst_e1;
+        destruct in_y_subst_e1 as [in_subst_es_1 | in_y_subst_e1].
+      tauto.
+      apply in_app_or in in_y_subst_e1;
+        destruct in_y_subst_e1 as [in_subst_es_1 | in_y_subst_e1];
+        tauto.
+
+subst_lfv_neq_rec_case.
+
+
+
+intros e1 x_nin_lfv_e1 in_y_subst_e1;
+  simpl in in_y_subst_e1;
+  apply_all e1 exp;
+  repeat (apply in_app_or in in_y_subst_e1;
+          destruct in_y_subst_e1 as [in_subst_es_1 | in_y_subst_e1];
+          match goal with
+          | [ IH : ?P1 -> ?P2 -> ?Q, H1 : ?P1, H2 : ?P2 |- ?Q ] =>
+            apply IH; assumption
+          end).
+    apply in_app_or in in_y_subst_e1.
+    destruct in_y_subst_e1 as [in_subst_es_1 | in_y_subst_e1].
+      match goal with
+          | [ IH : ?P1 -> ?P2 -> ?Q, H1 : ?P1, H2 : ?P2 |- ?Q ] =>
+            apply IH; assumption
+          end.
+    apply in_app_or in in_y_subst_e1.
+    destruct in_y_subst_e1 as [in_subst_es_1 | in_y_subst_e1].
+      match goal with
+          | [ IH : ?P1 -> ?P2 -> ?Q, H1 : ?P1, H2 : ?P2 |- ?Q ] =>
+            apply IH; assumption
+          end.
+
+  tauto.
+
+intros e1 x_nin_lfv_e1 in_y_subst_e1;
+       simpl in in_y_subst_e1;
+       apply in_app_or in in_y_subst_e1;
+       destruct in_y_subst_e1 as [in_subst_es_1 | in_y_subst_e1];
+       apply_all e1 exp.
+     repeat match goal with
+            | [ IH : ?P1 -> ?P2 -> ?Q, H1 : ?P1, H2 : ?P2 |- ?Q ] =>
+              apply IH; assumption
+            end.
+     apply in_app_or in in_y_subst_e1;
+       destruct in_y_subst_e1 as [in_subst_es_1 | in_y_subst_e1].
+     repeat match goal with
+            | [ IH : ?P1 -> ?P2 -> ?Q, H1 : ?P1, H2 : ?P2 |- ?Q ] =>
+              apply IH; assumption
+            end.
+     tauto.
+
+
+
+ intros e1 x_nin_lfv_e1 in_y_subst_e1.
+    simpl in in_y_subst_e1.
+    apply in_app_or in in_y_subst_e1;
+      destruct in_y_subst_e1 as [in_subst_es_1 | in_y_subst_e1].
+    + specialize (IHe2_2 e1).
+      firstorder.
+    +  apply in_app_or in in_y_subst_e1.
+       destruct in_y_subst_e1 as [in_subst_es_1 | in_y_subst_e1].
+       * apply (IHe2_2 e1); assumption.
+       * apply (IHe2_3 e1); assumption.
+  -
+
+Qed.
+
+Ltac apply_all e t:=
+  repeat match goal with
+         | [ H : forall ?e1 : t, _ |- _ ] =>
+           specialize (H e)
+         end.
+
+Ltac subst_lfv_neq_rec_case in_subst :=
+  intros e1 x_nin_lfv_e1 in_y_subst_e1;
+  simpl in in_y_subst_e1;
+  apply in_app_or in in_y_subst_e1;
+  destruct in_y_subst_e1 as [in_subst_es_1 | in_y_subst_e1];
+  apply_all e1 exp;
+  match goal with
+  | [ IH : ?P1 -> ?P2 -> ?Q, H1 : ?P1, H2 : ?P2 |- ?Q ] =>
+    apply IH; assumption
+  end.
+  
+  
+
+Lemma subst_lfv_neq' : forall x y e1 e2,
+    x <> y -> In y (lfv_exp (letsubst_exp e1 x e2)) -> 
+
+Ltac type_exp_no_lfv_rec_case :=
+  simpl;
+  repeat match goal with
+         | [ H : ?e1 = nil |- ?e1 ++ ?e2 = nil ] =>
+           rewrite H; simpl
+         end;
+  auto.
+
+Lemma notin_nil : forall {A : Set} (l : list A), (forall e, ~In e l) -> l = nil.
+Proof.
+  intros A l nin.
+  induction l.
+  - reflexivity.
+  - elim (nin a).
+    simpl; left; reflexivity.
+Qed.
+
+Lemma type_exp_no_lfv : forall g e t, type_exp g e t -> lfv_exp e = nil.
+Proof.
+  intros g e t te.
+  induction te.
+  all: try solve [auto | type_exp_no_lfv_rec_case].
+  - apply notin_nil.
+    simpl.
+    rewrite IHte1.
+    simpl.
+    intros e in_e_let.
+    rewrite in_list_minus in in_e_let.
+    destruct in_e_let.
+    
+    
+
+type_exp_no_lfv_rec_case.
+  -type_exp_no_lfv_rec_case.
+  -type_exp_no_lfv_rec_case.
+  -type_exp_no_lfv_rec_case.
+  all: type_exp_no_lfv_rec_case.
+  simpl in IHte2.
+
+Ltac var_in_fvs :=
+  try apply in_or_app;
+  first [ assumption | left; assumption | right; assumption | right; var_in_fvs].
+
+Ltac strengthen_rec_case C :=
+  apply C;
+  progress repeat match goal with
+  | [ H1 : ?P1, H2 : ~ In ?x _, IH : ?P1 -> ~ In ?x _ -> ?P2 |- ?P2 ] =>
+    apply IH; first [apply H1 | intro x_in; elim H2; simpl; var_in_fvs]
+  end.
+
+(*
+Lemma fv_subst_notin : forall x e e',
+    ~In x (fv_exp e) ->
+    ~In x (fv_exp (subst_exp e x e')).
+Proof.
+  intros x e e'.
+  remember (subst_exp e x e') as se.
+  induction se.
+  - intros ninxe.
+    destruct (eq_var var5 x).
+    rewrite e0 in Heqse.
+    
+      try (simpl in inxsubst; inversion inxsubst).
+      contradiction.
+  - intros e x nxe inxsubst.
+    simpl in inxsubst; inversion inxsubst.
+  - intros e x nxe inxsubst.
+    simpl in inxsubst.
+    apply in_app_or in inxsubst.
+    inversion inxsubst.
+    apply IHe'1.
+*)
+
+Lemma exp_strengthening : forall g e t x,
+    type_exp (cons x g) e t -> ~ In x (fv_exp e) -> type_exp g e t.
+Proof.
+  intros g e t x te n_in_fv.
+  fold gamma in g.
+  remember (x :: g) as g'.
+  induction te.
+  - rewrite Heqg' in H.
+    rewrite Heqg' in H0.
+    simpl in n_in_fv.
+    inversion H0.
+    inversion H.
+    + symmetry in H5.
+      elim n_in_fv.
+      left; assumption.
+    + apply t_var.
+      apply H5.
+      apply H4.
+  - rewrite Heqg' in H.
+    inversion H.
+    exact (t_int g num5 sz H3).
+  - strengthen_rec_case (t_load g e1 e2 ed sz nat5).
+  - strengthen_rec_case (t_store g e1 e2 ed sz e3).
+  - strengthen_rec_case (t_aop g e1 aop5 e2).
+  - strengthen_rec_case (t_lop g e1 lop5 e2 sz).
+  - strengthen_rec_case (t_uop g uop5 e1).
+  - strengthen_rec_case (t_cast g cast5 sz e nat5).
+  -
+  apply t_let.
+  progress repeat match goal with
+  | [ H1 : ?P1, H2 : ~ In ?x _, IH : ?P1 -> ~ In ?x _ -> ?P2 |- ?P2 ] =>
+    apply IH; first [apply H1 | intro x_in; elim H2; simpl]
+  end.
+  try apply in_or_app.
+  left; assumption.
+  progress repeat match goal with
+  | [ H1 : ?P1, H2 : ~ In ?x _, IH : ?P1 -> ~ In ?x _ -> ?P2 |- ?P2 ] =>
+    apply IH; first [apply H1 | intro x_in; elim H2; simpl]
+  end.
+  
+  try apply in_or_app.
+  right.
+
 
 Ltac exp_exchange_simple_base G :=
   match goal with
@@ -126,7 +511,6 @@ Ltac exp_exchange_simple_base G :=
           | apply tg_cons; assumption]
   end.
 
-Require Import Coq.Program.Equality.
 
 Lemma exp_exchange : forall id1 id2 t1 t2 g e t,
     id1 <> id2 ->
@@ -136,13 +520,12 @@ Lemma exp_exchange : forall id1 id2 t1 t2 g e t,
     type_exp ((var_var id2 t2) :: (var_var id1 t1) :: g) e t.
 Proof.
   intros id1 id2 t1 t2 g e t idneq id1_nin id2_nin te.
-  dependent induction te.
-
- (* remember ((var_var id1 t1) :: (var_var id2 t2) :: g) as G in te.*)
+  remember (var_var id1 t1 :: var_var id2 t2 :: g) as G12.
+  induction te.
   - apply t_var.
    (* rewrite HeqG in H. *)
     + simpl.
-      inversion H.
+      inversion H0.
       * right; left; assumption.
       * inversion H1.
         -- left; assumption.
